finish replacing rhssForNt calls with cache lookups

parser/Parser.v
@@ -49,6 +49,8 @@ Module ParserFn (Import D : Defs.T).
   | StepError  : parse_error -> step_result.
 
   Definition step (g  : grammar)
+                  (pm : production_map)
+                  (hc : production_map_correct pm g)
                   (cm : closure_map)
                   (ps : prefix_stack)
                   (ss : suffix_stack)
@@ -99,7 +101,7 @@ Module ParserFn (Import D : Defs.T).
       (* nonterminal case --> push a frame onto the stack *)
       | NT x :: _ => 
         if NtSet.mem x av then
-          match adaptivePredict g cm x ss ts ca with
+          match adaptivePredict g pm hc cm x ss ts ca with
           | (PredSucc rhs, ca') =>
             let ps' := (PF [] [], PF pre v :: p_frs)        in
             let ss' := (SF (Some x) rhs, SF o suf :: s_frs) in
@@ -121,27 +123,27 @@ Module ParserFn (Import D : Defs.T).
     end.
   
   Lemma step_StepAccept_facts :
-    forall g cm ps ss ts av un ca t,
-      step g cm ps ss ts av un ca = StepAccept t
+    forall g pm hc cm ps ss ts av un ca t,
+      step g pm hc cm ps ss ts av un ca = StepAccept t
       -> ts = []
          /\ exists o, ss = (SF o [], [])
          /\ exists pre,
              ps = (PF pre [t], []).
   Proof.
-    intros g cm ps ss ts av un ca v hs.
+    intros g pm hc cm ps ss ts av un ca v hs.
     unfold step in hs; dms; tc.
     inv hs; eauto.
   Qed.
 
   Lemma step_LeftRecursion_facts :
-    forall g cm ps ss ts av un ca x,
-      step g cm ps ss ts av un ca = StepError (LeftRecursion x)
+    forall g pm hc cm ps ss ts av un ca x,
+      step g pm hc cm ps ss ts av un ca = StepError (LeftRecursion x)
       -> ~ NtSet.In x av
          /\ NtSet.In x (allNts g)
          /\ exists o suf frs,
              ss = (SF o (NT x :: suf), frs).
   Proof.
-    intros g cm ps ss ts av un ca x hs.
+    intros g cm pm hc ps ss ts av un ca x hs.
     unfold step in hs; repeat dmeq h; tc; inv hs; sis;
       repeat split; eauto.
     - unfold not; intros hi; apply NF.mem_iff in hi; tc.
@@ -149,12 +151,12 @@ Module ParserFn (Import D : Defs.T).
   Qed.
 
   Lemma step_preserves_cache_invar :
-    forall g cm ps ps' ss ss' ts ts' av av' un un' ca ca',
-      cache_stores_target_results g cm ca
-      -> step g cm ps ss ts av un ca = StepK ps' ss' ts' av' un' ca'
-      -> cache_stores_target_results g cm ca'.
+    forall g pm hc cm ps ps' ss ss' ts ts' av av' un un' ca ca',
+      cache_stores_target_results g pm hc cm ca
+      -> step g pm hc cm ps ss ts av un ca = StepK ps' ss' ts' av' un' ca'
+      -> cache_stores_target_results g pm hc cm ca'.
   Proof.
-    intros gr cm ps ps' ss ss' ts ts' av av' un un' ca ca' hc hs.
+    intros gr pm hpc cm ps ps' ss ss' ts ts' av av' un un' ca ca' hc hs.
     unfold step in hs; dmeqs H; tc; inv hs; auto.
     - eapply adaptivePredict_succ_preserves_cache_invar;  eauto.
     - eapply adaptivePredict_ambig_preserves_cache_invar; eauto.
@@ -199,12 +201,12 @@ Module ParserFn (Import D : Defs.T).
   Defined.
 
   Lemma step_meas_lt :
-    forall g cm ps ps' ss ss' ts ts' av av' un un' ca ca',
-      cache_stores_target_results g cm ca
-      -> step g cm ps ss ts av un ca = StepK ps' ss' ts' av' un' ca'
+    forall g pm hc cm ps ps' ss ss' ts ts' av av' un un' ca ca',
+      cache_stores_target_results g pm hc cm ca
+      -> step g pm hc cm ps ss ts av un ca = StepK ps' ss' ts' av' un' ca'
       -> lex_nat_triple (meas g ss' ts' av') (meas g ss ts av).
   Proof.
-    intros g cm ps ps' ss ss' ts ts' av av' un un' ca ca' hc hs; unfold step in hs.
+    intros g pm hpc cm ps ps' ss ss' ts ts' av av' un un' ca ca' hc hs; unfold step in hs.
     destruct ss as ([ o [| [a|x] suf] ], frs).
     - dms; tc; inv hs.
       eapply meas_lt_after_return; eauto.
@@ -221,9 +223,9 @@ Module ParserFn (Import D : Defs.T).
   Qed.
 
   Lemma StepK_result_acc :
-    forall g cm ps ps' ss ss' ts ts' av av' un un' ca ca' (a : Acc lex_nat_triple (meas g ss ts av)),
-      cache_stores_target_results g cm ca
-      -> step g cm ps ss ts av un ca = StepK ps' ss' ts' av' un' ca'
+    forall g pm hc cm ps ps' ss ss' ts ts' av av' un un' ca ca' (a : Acc lex_nat_triple (meas g ss ts av)),
+      cache_stores_target_results g pm hc cm ca
+      -> step g pm hc cm ps ss ts av un ca = StepK ps' ss' ts' av' un' ca'
       -> Acc lex_nat_triple (meas g ss' ts' av').
   Proof.
     intros; eapply Acc_inv; eauto.
@@ -231,6 +233,8 @@ Module ParserFn (Import D : Defs.T).
   Defined.
   
   Fixpoint multistep (gr : grammar)
+                     (pm : production_map)
+                     (hp : production_map_correct pm gr)
                      (cm : closure_map)
                      (ps : prefix_stack)
                      (ss : suffix_stack)
@@ -238,30 +242,30 @@ Module ParserFn (Import D : Defs.T).
                      (av : NtSet.t)
                      (un : bool)
                      (ca : cache)
-                     (hc : cache_stores_target_results gr cm ca)
+                     (hc : cache_stores_target_results gr pm hp cm ca)
                      (ha : Acc lex_nat_triple (meas gr ss ts av))
                      {struct ha} : parse_result :=
-    match step gr cm ps ss ts av un ca as res return step gr cm ps ss ts av un ca = res -> _ with
+    match step gr pm hp cm ps ss ts av un ca as res return step gr pm hp cm ps ss ts av un ca = res -> _ with
     | StepAccept v                  => fun _  => if un then Accept v else Ambig v
     | StepReject s                  => fun _  => Reject s
     | StepError e                   => fun _  => Error e
     | StepK ps' ss' ts' av' un' ca' =>
-      fun hs => multistep gr cm ps' ss' ts' av' un' ca'
-                          (step_preserves_cache_invar _ _ _ _ _ _ _ _ _ _ _ _ _ _ hc hs)
-                          (StepK_result_acc _ _ _ _ _ _ _ _ _ _ _ _ _ _ ha hc hs)
+      fun hs => multistep gr pm hp cm ps' ss' ts' av' un' ca'
+                          (step_preserves_cache_invar _ _ _ _ _ _ _ _ _ _ _ _ _ _ _ _ hc hs)
+                          (StepK_result_acc _ _ _ _ _ _ _ _ _ _ _ _ _ _ _ _ ha hc hs)
     end eq_refl.
 
   Lemma multistep_unfold :
-    forall gr cm ps ss ts av un ca hc ha,
-      multistep gr cm ps ss ts av un ca hc ha =
-      match step gr cm ps ss ts av un ca as res return step gr cm ps ss ts av un ca = res -> _ with
+    forall gr pm hp cm ps ss ts av un ca hc ha,
+      multistep gr pm hp cm ps ss ts av un ca hc ha =
+      match step gr pm hp cm ps ss ts av un ca as res return step gr pm hp cm ps ss ts av un ca = res -> _ with
       | StepAccept v                  => fun _  => if un then Accept v else Ambig v
       | StepReject s                  => fun _  => Reject s
       | StepError e                   => fun _  => Error e
       | StepK ps' ss' ts' av' un' ca' =>
-        fun hs => multistep gr cm ps' ss' ts' av' un' ca'
-                            (step_preserves_cache_invar _ _ _ _ _ _ _ _ _ _ _ _ _ _ hc hs)
-                            (StepK_result_acc _ _ _ _ _ _ _ _ _ _ _ _ _ _ ha hc hs)
+        fun hs => multistep gr pm hp cm ps' ss' ts' av' un' ca'
+                            (step_preserves_cache_invar _ _ _ _ _ _ _ _ _ _ _ _ _ _ _ _ hc hs)
+                            (StepK_result_acc _ _ _ _ _ _ _ _ _ _ _ _ _ _ _ _ ha hc hs)
       end eq_refl.
   Proof.
     intros; destruct ha; auto.
@@ -269,6 +273,8 @@ Module ParserFn (Import D : Defs.T).
   
   Lemma multistep_cases' :
     forall (gr  : grammar)
+           (pm  : production_map)
+           (hp  : production_map_correct pm gr)
            (cm  : closure_map)
            (ps  : prefix_stack)
            (ss  : suffix_stack)
@@ -276,46 +282,48 @@ Module ParserFn (Import D : Defs.T).
            (av  : NtSet.t)
            (un  : bool)
            (ca  : cache)
-           (hc  : cache_stores_target_results gr cm ca)
+           (hc  : cache_stores_target_results gr pm hp cm ca)
            (ha  : Acc lex_nat_triple (meas gr ss ts av))
            (sr  : step_result)
            (pr  : parse_result)
-           (heq : step gr cm ps ss ts av un ca = sr),
-      match sr as res return (step gr cm ps ss ts av un ca = res -> parse_result) with
+           (heq : step gr pm hp cm ps ss ts av un ca = sr),
+      match sr as res return (step gr pm hp cm ps ss ts av un ca = res -> parse_result) with
       | StepAccept sv                 => fun _ => if un then Accept sv else Ambig sv
       | StepReject s                  => fun _ => Reject s
       | StepError s                   => fun _ => Error s
       | StepK ps' ss' ts' av' un' ca' =>
-        fun hs => multistep gr cm ps' ss' ts' av' un' ca'
-                            (step_preserves_cache_invar _ _ _ _ _ _ _ _ _ _ _ _ _ _ hc hs)
-                            (StepK_result_acc _ _ _ _ _ _ _ _ _ _ _ _ _ _ ha hc hs)
+        fun hs => multistep gr pm hp cm ps' ss' ts' av' un' ca'
+                            (step_preserves_cache_invar _ _ _ _ _ _ _ _ _ _ _ _ _ _ _ _ hc hs)
+                            (StepK_result_acc _ _ _ _ _ _ _ _ _ _ _ _ _ _ _ _ ha hc hs)
       end heq = pr
       -> match pr with
          | Accept f => (sr = StepAccept f /\ un = true)
                        \/ (exists ps' ss' ts' av' un' ca' hc' ha',
                               sr = StepK ps' ss' ts' av' un' ca'
-                              /\ multistep gr cm ps' ss' ts' av' un' ca' hc' ha' = Accept f)
+                              /\ multistep gr pm hp cm ps' ss' ts' av' un' ca' hc' ha' = Accept f)
          | Ambig f  => (sr = StepAccept f /\ un = false)
                        \/ (exists ps' ss' ts' av' un' ca' hc' ha',
                               sr = StepK ps' ss' ts' av' un' ca'
-                              /\ multistep gr cm ps' ss' ts' av' un' ca' hc' ha' = Ambig f)
+                              /\ multistep gr pm hp cm ps' ss' ts' av' un' ca' hc' ha' = Ambig f)
          | Reject s => sr = StepReject s
                        \/ (exists ps' ss' ts' av' un' ca' hc' ha',
                               sr = StepK ps' ss' ts' av' un' ca'
-                              /\ multistep gr cm ps' ss' ts' av' un' ca' hc' ha' = Reject s)
+                              /\ multistep gr pm hp cm ps' ss' ts' av' un' ca' hc' ha' = Reject s)
          | Error s  => sr = StepError s
                        \/ (exists ps' ss' ts' av' un' ca' hc' ha',
                               sr = StepK ps' ss' ts' av' un' ca'
-                              /\ multistep gr cm ps' ss' ts' av' un' ca' hc' ha' = Error s)
+                              /\ multistep gr pm hp cm ps' ss' ts' av' un' ca' hc' ha' = Error s)
          end.
   Proof.
-    intros g cm ps ss ts av un ca hc ha sr pr heq.
+    intros g pm hp cm ps ss ts av un ca hc ha sr pr heq.
     destruct pr; destruct sr; destruct un;
       try solve [ intros; tc | intros h; inv h; auto | intros h; right; eauto 10].
   Qed.
 
   Lemma multistep_cases :
     forall (gr  : grammar)
+           (pm  : production_map)
+           (hp  : production_map_correct pm gr)
            (cm  : closure_map)
            (ps  : prefix_stack)
            (ss  : suffix_stack)
@@ -323,36 +331,38 @@ Module ParserFn (Import D : Defs.T).
            (av  : NtSet.t)
            (un  : bool)
            (ca  : cache)
-           (hc  : cache_stores_target_results gr cm ca)
+           (hc  : cache_stores_target_results gr pm hp cm ca)
            (ha  : Acc lex_nat_triple (meas gr ss ts av))
            (pr  : parse_result),
-      multistep gr cm ps ss ts av un ca hc ha = pr
+      multistep gr pm hp cm ps ss ts av un ca hc ha = pr
       -> match pr with
-         | Accept f => (step gr cm ps ss ts av un ca = StepAccept f /\ un = true)
+         | Accept f => (step gr pm hp cm ps ss ts av un ca = StepAccept f /\ un = true)
                        \/ (exists ps' ss' ts' av' un' ca' hc' ha',
-                              step gr cm ps ss ts av un ca = StepK ps' ss' ts' av' un' ca'
-                              /\ multistep gr cm ps' ss' ts' av' un' ca' hc' ha' = Accept f)
-         | Ambig f  => (step gr cm ps ss ts av un ca = StepAccept f /\ un = false)
+                              step gr pm hp cm ps ss ts av un ca = StepK ps' ss' ts' av' un' ca'
+                              /\ multistep gr pm hp cm ps' ss' ts' av' un' ca' hc' ha' = Accept f)
+         | Ambig f  => (step gr pm hp cm ps ss ts av un ca = StepAccept f /\ un = false)
                        \/ (exists ps' ss' ts' av' un' ca' hc' ha',
-                              step gr cm ps ss ts av un ca = StepK ps' ss' ts' av' un' ca'
-                              /\ multistep gr cm ps' ss' ts' av' un' ca' hc' ha' = Ambig f)
-         | Reject s => step gr cm ps ss ts av un ca = StepReject s
+                              step gr pm hp cm ps ss ts av un ca = StepK ps' ss' ts' av' un' ca'
+                              /\ multistep gr pm hp cm ps' ss' ts' av' un' ca' hc' ha' = Ambig f)
+         | Reject s => step gr pm hp cm ps ss ts av un ca = StepReject s
                        \/ (exists ps' ss' ts' av' un' ca' hc' ha',
-                              step gr cm ps ss ts av un ca = StepK ps' ss' ts' av' un' ca'
-                              /\ multistep gr cm ps' ss' ts' av' un' ca' hc' ha' = Reject s)
-         | Error s  => step gr cm ps ss ts av un ca = StepError s
+                              step gr pm hp cm ps ss ts av un ca = StepK ps' ss' ts' av' un' ca'
+                              /\ multistep gr pm hp cm ps' ss' ts' av' un' ca' hc' ha' = Reject s)
+         | Error s  => step gr pm hp cm ps ss ts av un ca = StepError s
                        \/ (exists ps' ss' ts' av' un' ca' hc' ha',
-                              step gr cm ps ss ts av un ca = StepK ps' ss' ts' av' un' ca'
-                              /\ multistep gr cm ps' ss' ts' av' un' ca' hc' ha' = Error s)
+                              step gr pm hp cm ps ss ts av un ca = StepK ps' ss' ts' av' un' ca'
+                              /\ multistep gr pm hp cm ps' ss' ts' av' un' ca' hc' ha' = Error s)
          end.
   Proof.
-    intros g cm ps ss ts av un ca hc ha pr hm; subst.
+    intros g pm hp cm ps ss ts av un ca hc ha pr hm; subst.
     rewrite multistep_unfold.
     eapply multistep_cases'; eauto.
   Qed.
 
   Lemma multistep_accept_cases :
     forall (gr : grammar)
+           (pm  : production_map)
+           (hp  : production_map_correct pm gr)
            (cm : closure_map)
            (ps : prefix_stack)
            (ss : suffix_stack)
@@ -360,21 +370,23 @@ Module ParserFn (Import D : Defs.T).
            (av : NtSet.t)
            (un : bool)
            (ca : cache)
-           (hc : cache_stores_target_results gr cm ca)
+           (hc : cache_stores_target_results gr pm hp cm ca)
            (ha : Acc lex_nat_triple (meas gr ss ts av))
            (t  : tree),
-      multistep gr cm ps ss ts av un ca hc ha = Accept t
-      -> (step gr cm ps ss ts av un ca = StepAccept t /\ un = true)
+      multistep gr pm hp cm ps ss ts av un ca hc ha = Accept t
+      -> (step gr pm hp cm ps ss ts av un ca = StepAccept t /\ un = true)
          \/ (exists ps' ss' ts' av' un' ca' hc' ha',
-                step gr cm ps ss ts av un ca = StepK ps' ss' ts' av' un' ca'
-                /\ multistep gr cm ps' ss' ts' av' un' ca' hc' ha' = Accept t).
+                step gr pm hp cm ps ss ts av un ca = StepK ps' ss' ts' av' un' ca'
+                /\ multistep gr pm hp cm ps' ss' ts' av' un' ca' hc' ha' = Accept t).
   Proof.
-    intros ? ? ? ? ? ? ? ? ? ? ? hm; subst. 
-    destruct (multistep_cases _ _ _ _ _ _ _ _ _ _ _ hm); auto.
+    intros ? ? ? ? ? ? ? ? ? ? ? ? ? hm; subst. 
+    destruct (multistep_cases _ _ _ _ _ _ _ _ _ _ _ _ _ hm); auto.
   Qed.
 
   Lemma multistep_ambig_cases :
     forall (gr : grammar)
+           (pm : production_map)
+           (hp : production_map_correct pm gr)
            (cm : closure_map)
            (ps : prefix_stack)
            (ss : suffix_stack)
@@ -382,21 +394,24 @@ Module ParserFn (Import D : Defs.T).
            (av : NtSet.t)
            (un : bool)
            (ca : cache)
-           (hc : cache_stores_target_results gr cm ca)
+           (hc : cache_stores_target_results gr pm hp cm ca)
            (ha : Acc lex_nat_triple (meas gr ss ts av))
            (t  : tree),
-      multistep gr cm ps ss ts av un ca hc ha = Ambig t 
-      -> (step gr cm ps ss ts av un ca = StepAccept t /\ un = false)
+      multistep gr pm hp cm ps ss ts av un ca hc ha = Ambig t 
+      -> (step gr pm hp cm ps ss ts av un ca = StepAccept t /\ un = false)
          \/ (exists ps' ss' ts' av' un' ca' hc' ha',
-                step gr cm ps ss ts av un ca = StepK ps' ss' ts' av' un' ca'
-                /\ multistep gr cm ps' ss' ts' av' un' ca' hc' ha' = Ambig t).
+                step gr pm hp cm ps ss ts av un ca = StepK ps' ss' ts' av' un' ca'
+                /\ multistep gr pm hp cm ps' ss' ts' av' un' ca' hc' ha' = Ambig t).
+
   Proof.
-    intros ? ? ? ? ? ? ? ? ? ? ? hm; subst. 
-    destruct (multistep_cases _ _ _ _ _ _ _ _ _ _ _ hm); auto.
+    intros ? ? ? ? ? ? ? ? ? ? ? ? ? hm; subst. 
+    destruct (multistep_cases _ _ _ _ _ _ _ _ _ _ _ _ _ hm); auto.
   Qed.
 
   Lemma multistep_reject_cases :
     forall (gr : grammar)
+           (pm : production_map)
+           (hp : production_map_correct pm gr)
            (cm : closure_map)
            (ps : prefix_stack)
            (ss : suffix_stack)
@@ -404,21 +419,23 @@ Module ParserFn (Import D : Defs.T).
            (av : NtSet.t)
            (un : bool)
            (ca : cache)
-           (hc : cache_stores_target_results gr cm ca)
+           (hc : cache_stores_target_results gr pm hp cm ca)
            (ha : Acc lex_nat_triple (meas gr ss ts av))
            (s  : string),
-      multistep gr cm ps ss ts av un ca hc ha = Reject s
-      -> step gr cm ps ss ts av un ca = StepReject s
+      multistep gr pm hp cm ps ss ts av un ca hc ha = Reject s
+      -> step gr pm hp cm ps ss ts av un ca = StepReject s
          \/ (exists ps' ss' ts' av' un' ca' hc' ha',
-                step gr cm ps ss ts av un ca = StepK ps' ss' ts' av' un' ca'
-                /\ multistep gr cm ps' ss' ts' av' un' ca' hc' ha' = Reject s).
+                step gr pm hp cm ps ss ts av un ca = StepK ps' ss' ts' av' un' ca'
+                /\ multistep gr pm hp cm ps' ss' ts' av' un' ca' hc' ha' = Reject s).
   Proof.
-    intros ? ? ? ? ? ? ? ? ? ? ? hm; subst. 
-    destruct (multistep_cases _ _ _ _ _ _ _ _ _ _ _ hm); auto.
+    intros ? ? ? ? ? ? ? ? ? ? ? ? ? hm; subst. 
+    destruct (multistep_cases _ _ _ _ _ _ _ _ _ _ _ _ _ hm); auto.
   Qed.
 
   Lemma multistep_invalid_state_cases :
     forall (gr : grammar)
+           (pm : production_map)
+           (hp : production_map_correct pm gr)
            (cm : closure_map)
            (ps : prefix_stack)
            (ss : suffix_stack)
@@ -426,20 +443,22 @@ Module ParserFn (Import D : Defs.T).
            (av : NtSet.t)
            (un : bool)
            (ca : cache)
-           (hc : cache_stores_target_results gr cm ca)
+           (hc : cache_stores_target_results gr pm hp cm ca)
            (ha : Acc lex_nat_triple (meas gr ss ts av)),
-      multistep gr cm ps ss ts av un ca hc ha = Error InvalidState
-      -> step gr cm ps ss ts av un ca = StepError InvalidState
+      multistep gr pm hp cm ps ss ts av un ca hc ha = Error InvalidState
+      -> step gr pm hp cm ps ss ts av un ca = StepError InvalidState
          \/ (exists ps' ss' ts' av' un' ca' hc' ha',
-                step gr cm ps ss ts av un ca = StepK ps' ss' ts' av' un' ca'
-                /\ multistep gr cm ps' ss' ts' av' un' ca' hc' ha' = Error InvalidState).
+                step gr pm hp cm ps ss ts av un ca = StepK ps' ss' ts' av' un' ca'
+                /\ multistep gr pm hp cm ps' ss' ts' av' un' ca' hc' ha' = Error InvalidState).
   Proof.
-    intros ? ? ? ? ? ? ? ? ? ? hm; subst.
-    destruct (multistep_cases _ _ _ _ _ _ _ _ _ _ _ hm); auto.
+    intros ? ? ? ? ? ? ? ? ? ? ? ? hm; subst.
+    destruct (multistep_cases _ _ _ _ _ _ _ _ _ _ _ _ _ hm); auto.
   Qed.
 
   Lemma multistep_left_recursion_cases :
     forall (gr : grammar)
+           (pm : production_map)
+           (hp : production_map_correct pm gr)
            (cm : closure_map)
            (ps : prefix_stack)
            (ss : suffix_stack)
@@ -447,21 +466,23 @@ Module ParserFn (Import D : Defs.T).
            (av : NtSet.t)
            (un : bool)
            (ca : cache)
-           (hc : cache_stores_target_results gr cm ca)
+           (hc : cache_stores_target_results gr pm hp cm ca)
            (ha : Acc lex_nat_triple (meas gr ss ts av))
            (x  : nonterminal),
-      multistep gr cm ps ss ts av un ca hc ha = Error (LeftRecursion x)
-      -> step gr cm ps ss ts av un ca = StepError (LeftRecursion x)
+      multistep gr pm hp cm ps ss ts av un ca hc ha = Error (LeftRecursion x)
+      -> step gr pm hp cm ps ss ts av un ca = StepError (LeftRecursion x)
          \/ (exists ps' ss' ts' av' un' ca' hc' ha',
-                step gr cm ps ss ts av un ca = StepK ps' ss' ts' av' un' ca'
-                /\ multistep gr cm ps' ss' ts' av' un' ca' hc' ha' = Error (LeftRecursion x)).
+                step gr pm hp cm ps ss ts av un ca = StepK ps' ss' ts' av' un' ca'
+                /\ multistep gr pm hp cm ps' ss' ts' av' un' ca' hc' ha' = Error (LeftRecursion x)).
   Proof.
-    intros ? ? ? ? ? ? ? ? ? ? ? hm; subst.
-    destruct (multistep_cases _ _ _ _ _ _ _ _ _ _ _ hm); auto.
+    intros ? ? ? ? ? ? ? ? ? ? ? ? ? hm; subst.
+    destruct (multistep_cases _ _ _ _ _ _ _ _ _ _ _ _ _ hm); auto.
   Qed.
 
   Lemma multistep_prediction_error_cases :
     forall (gr : grammar)
+           (pm : production_map)
+           (hp : production_map_correct pm gr)
            (cm : closure_map)
            (ps : prefix_stack)
            (ss : suffix_stack)
@@ -469,35 +490,37 @@ Module ParserFn (Import D : Defs.T).
            (av : NtSet.t)
            (un : bool)
            (ca : cache)
-           (hc : cache_stores_target_results gr cm ca)
+           (hc : cache_stores_target_results gr pm hp cm ca)
            (ha : Acc lex_nat_triple (meas gr ss ts av))
            (e  : prediction_error),
-      multistep gr cm ps ss ts av un ca hc ha = Error (PredictionError e)
-      -> step gr cm ps ss ts av un ca = StepError (PredictionError e)
+      multistep gr pm hp cm ps ss ts av un ca hc ha = Error (PredictionError e)
+      -> step gr pm hp cm ps ss ts av un ca = StepError (PredictionError e)
          \/ (exists ps' ss' ts' av' un' ca' hc' ha',
-                step gr cm ps ss ts av un ca = StepK ps' ss' ts' av' un' ca'
-                /\ multistep gr cm ps' ss' ts' av' un' ca' hc' ha' = Error (PredictionError e)).
+                step gr pm hp cm ps ss ts av un ca = StepK ps' ss' ts' av' un' ca'
+                /\ multistep gr pm hp cm ps' ss' ts' av' un' ca' hc' ha' = Error (PredictionError e)).
   Proof.
-    intros ? ? ? ? ? ? ? ? ? ? ? hm; subst.
-    destruct (multistep_cases _ _ _ _ _ _ _ _ _ _ _ hm); auto.
+    intros ? ? ? ? ? ? ? ? ? ? ? ? ? hm; subst.
+    destruct (multistep_cases _ _ _ _ _ _ _ _ _ _ _ _ _ hm); auto.
   Qed.
 
   Lemma empty_cache_stores_target_results :
-    forall gr cm,
-      cache_stores_target_results gr cm empty_cache.
+    forall gr pm hp cm,
+      cache_stores_target_results gr pm hp cm empty_cache.
   Proof.
-    intros gr cm sps a sps' hf.
+    intros gr pm hp cm sps a sps' hf.
     rewrite CacheFacts.empty_o in hf; tc.
   Defined.
 
   (* This curried pattern enables us to partially apply the parser to a grammar
      and compute the closure map once, instead of each time we parse an input *)
   Definition parse (g : grammar) : nonterminal -> list token -> parse_result :=
-    let cm := mkClosureMap g in
+    let pm := mkProductionMap g         in
+    let hp := mkProductionMap_correct g in
+    let cm := mkClosureMap g            in
     fun (x : nonterminal) (ts : list token) =>
       let p_stk0 := (PF []   []    , []) in
       let s_stk0 := (SF None [NT x], []) in
-      multistep g cm p_stk0 s_stk0 ts (allNts g) true empty_cache
-                (empty_cache_stores_target_results g cm) (lex_nat_triple_wf _).
+      multistep g pm hp cm p_stk0 s_stk0 ts (allNts g) true empty_cache
+                (empty_cache_stores_target_results g pm hp cm) (lex_nat_triple_wf _).
 
 End ParserFn.
